src/syntax.mli
@@ -70,7 +70,7 @@ type rec_type =
   | Structural of Id.t located option
   | Logical of rec_info
 and rec_info = {
-  comp : constant;
+  comp : constant option;
   comp_app : constr;
   comp_proj : constant;
   comp_recarg : int;
